theories/examples/spinlock/spinlock_proof.v
@@ -1,14 +1,15 @@
+From iris.algebra Require Import csum excl auth cmra_big_op.
+From iris.algebra Require Import big_op gset frac agree.
 From refinedc.typing Require Import typing.
 From refinedc.examples.spinlock Require Import spinlock_def.
 From refinedc.examples.spinlock Require Import spinlock_spec.
 From refinedc.examples.spinlock Require Import spinlock_code.
-From iris.algebra Require Import csum excl auth cmra_big_op.
-From iris.algebra Require Import big_op gset frac agree.
 Set Default Proof Using "Type".
 
 Section type.
   Context `{!typeG Σ} `{!lockG Σ}.
   Typeclasses Transparent spinlock spinlocked_ex spinlock_token spinlocked_ex_token.
+
 
   Lemma type_sl_init:
     ⊢ typed_function impl_sl_init type_of_sl_init.
@@ -17,13 +18,12 @@ Section type.
 
     iApply fupd_typed_stmt.
     iMod (own_alloc (● GSet ∅)) as (γ) "Hown". by apply auth_auth_valid.
+    iAssert (spinlock_token γ []) with "[Hown]" as "?". iExists _. by iFrame.
     iModIntro.
 
     repeat liRStep; liShow.
-    iIntros "?". rewrite /(ty_own (spinlock _))/=.
     liInst Hevar γ.
     repeat liRStep; liShow.
-    iSplitL => //. iExists _. by iFrame.
     Unshelve. all: prepare_sideconditions; solve_goal.
   Qed.
 
@@ -35,63 +35,8 @@ Section type.
 
     - repeat liRStep; liShow.
     - repeat liRStep; liShow.
-      iApply typed_place_subsume'.
-      destruct β.
-      + iDestruct 1 as (b) "[? ?]".
-        repeat liRStep; liShow.
-        iIntros "H1 H2 H3" (Φ) "HΦ".
-        iDestruct "H1" as (_) "H1".
-        iDestruct "H2" as (_) "H2".
-        (* TODO: don't unfold here *)
-        rewrite {2 3}/boolean/boolean_inner_type/int_inner_type/=.
-        iDestruct "H1" as (vo Hvo Hlo) "Ho" => /=. iDestruct "H2" as (ve Hve Hle) "He" => /=.
-        destruct b.
-        * iApply (wp_cas_fail with "Ho He"); try by [apply val_to_of_loc]; try by [apply val_to_of_int].
-          all: try by rewrite // /loc_size/loc_size_log/it_length/it_size/=; lia.
-          iIntros "!# Hvo Hve".
-          iApply ("HΦ" $! _ (t2mt (Z_of_bool false @ int bool_it))%I with "[]") => //.
-          iAssert (p at{struct_spinlock}ₗ "lock" ◁ₗ true @ boolean u8)%I with "[Hvo]" as "Hp". by iExists _; iFrame.
-          iAssert (vexpected ◁ₗ true @ boolean u8)%I with "[Hve]" as "He". by iExists _; iFrame.
-          repeat liRStep; liShow.
-          iIntros "?". rewrite /(ty_own (spinlock _))/=.
-          repeat liRStep; liShow.
-        * iApply (wp_cas_suc with "Ho He"); try by [apply val_to_of_loc]; try by [apply val_to_of_int].
-          all: try by rewrite // /loc_size/loc_size_log/it_length/it_size/=; lia.
-          iIntros "!# Hvo Hve".
-          iApply ("HΦ" $! _ (t2mt (Z_of_bool true @ int bool_it))%I with "[]") => //.
-          iAssert (p at{struct_spinlock}ₗ "lock" ◁ₗ true @ boolean u8)%I with "[Hvo]" as "Hp". by iExists _; iFrame.
-          iAssert (vexpected ◁ₗ false @ boolean u8)%I with "[Hve]" as "He". by iExists _; iFrame.
-          repeat liRStep; liShow.
-          iIntros "?". rewrite /(ty_own (spinlock _))/=.
-          repeat liRStep; liShow.
-      + iIntros "[% [#? #Hinv]]".
-        repeat liRStep; liShow.
-        iIntros "H1 H2 H3" (Φ) "HΦ". iDestruct "H2" as (_) "H2".
-        (* TODO: don't unfold here *)
-        rewrite {2}/boolean/boolean_inner_type/int_inner_type/=. iDestruct "H2" as (ve Hve Hle) "He" => /=.
-        iApply (@wp_atomic).
-        iMod (inv_acc with "Hinv") as "[Hb Hc]" => //. iModIntro.
-        iDestruct "Hb" as (b) "[>Hmt Hown]".
-        destruct b.
-        * iApply (wp_cas_fail with "Hmt He"); try by [apply val_to_of_loc]; try by [apply val_to_of_int]; try by [apply val_to_int_bool].
-          all: try by rewrite // /loc_size/loc_size_log/it_length/it_size/=; lia.
-          iIntros "!# Hl He".
-          iMod ("Hc" with "[Hl]") as "_"; iModIntro. by iExists _; iFrame.
-          iApply ("HΦ" $! _ (t2mt (Z_of_bool false @ int bool_it))%I with "[]") => //.
-          iAssert (vexpected ◁ₗ true @ boolean u8)%I with "[He]" as "He". by iExists _; iFrame.
-          repeat liRStep; liShow.
-          iIntros "?". rewrite /(ty_own (spinlock _))/=.
-          repeat liRStep; liShow.
-        * iApply (wp_cas_suc with "Hmt He"); try by [apply val_to_of_loc]; try by [apply val_to_of_int]; try by [apply val_to_int_bool].
-          all: try by rewrite // /loc_size/loc_size_log/it_length/it_size/=; lia.
-          iIntros "!# Hl He".
-          iMod ("Hc" with "[Hl]") as "_"; iModIntro. rewrite/val_of_bool. by iExists true => /=; iFrame.
-          iApply ("HΦ" $! _ (t2mt (Z_of_bool true @ int bool_it))%I with "[]") => //.
-          iAssert (vexpected ◁ₗ false @ boolean u8)%I with "[He]" as "He". by iExists _; iFrame.
-          repeat liRStep; liShow.
-          iIntros "?". rewrite /(ty_own (spinlock _))/=.
-          repeat liRStep; liShow.
-          Unshelve. all: prepare_sideconditions; solve_goal.
+      Unshelve. all: prepare_sideconditions; try solve_goal.
+      rewrite /it_length/=. have ->: loc_size = 8%nat; solve_goal.
   Qed.
 
   Lemma type_sl_unlock:
@@ -100,27 +45,7 @@ Section type.
     start_function "sl_unlock" ([[p γ] β]) => vl. split_blocks (∅ : gmap block_id (iProp Σ)) (∅ : gmap block_id (iProp Σ)).
 
     repeat liRStep; liShow.
-    iApply typed_place_subsume'.
-    destruct β.
-    - iDestruct 1 as (b) "[? ?]".
-      repeat liRStep; liShow.
-      iIntros "?". rewrite /(ty_own (spinlock _))/=.
-      repeat liRStep; liShow.
-    - iIntros "[% [#? #Hinv]]".
-      repeat liRStep; liShow.
-      iExists (_, singleton_place _)%I => /=. iSplit => //.
-      iIntros "_" => /=.
-      iMod (inv_acc with "Hinv") as "[Hl Hc]" => //.
-      iDestruct "Hl" as (b) "[>Hb Hown]".
-      iMod (fupd_intro_mask') as "Hmask". 2: iModIntro. solve_ndisj.
-      iSplitL "Hb". by iExists _; iFrame; iPureIntro; destruct b.
-      iIntros "!# Hp _".
-      iMod "Hmask" as "_". iMod ("Hc" with "[-]"). rewrite /val_of_bool. by iModIntro; iExists false; iFrame.
-      iIntros "!#". iExists (singleton_place (p at{struct_spinlock}ₗ "lock"))%I. iSplit => //.
-      repeat liRStep; liShow.
-      iIntros "?". rewrite /(ty_own (spinlock _))/=.
-      repeat liRStep; liShow.
-      Unshelve. all: prepare_sideconditions; solve_goal.
+    Unshelve. all: prepare_sideconditions; solve_goal.
   Qed.
 
 End type.
