theories/typing/atomic_bool.v
@@ -1,0 +1,157 @@
+From refinedc.typing Require Export type.
+From refinedc.typing Require Import programs int.
+Set Default Proof Using "Type".
+
+Definition atomic_boolN : namespace := nroot.@"atomic_boolN".
+Section atomic_bool.
+  Context `{!typeG Σ}.
+
+  Program Definition atomic_bool (it : int_type) (PT PF : iProp Σ) : type := {|
+    ty_own β l := (match β return _ with
+                  | Own => ∃ b, l ◁ₗ b @ boolean it ∗ if b then PT else PF
+                  | Shr => ⌜l `has_layout_loc` it⌝ ∗
+                          inv atomic_boolN (∃ b, l ↦ i2v (Z_of_bool b) it ∗ if b then PT else PF)
+                  end)%I
+  |}.
+  Next Obligation.
+    iIntros (PT PF l E HE) => /=. iDestruct 1 as (b) "[Hb Hown]".
+    iDestruct (ty_aligned with "Hb") as %?. iSplitR => //.
+    iApply inv_alloc. iIntros "!#". iExists b. iFrame.
+    iDestruct (ty_deref with "Hb") as (v) "[Hl Hb]".
+    (* TODO: don't unfold here *)
+    rewrite /i2v. by iDestruct "Hb" as %->.
+  Qed.
+
+  Global Program Instance movable_atomic_bool it PT PF : Movable (atomic_bool it PT PF) := {|
+    ty_layout := it_layout it;
+    ty_own_val v := ∃ b, v ◁ᵥ b @ boolean it ∗ if b then PT else PF;
+  |}%I.
+  Next Obligation. iIntros (it PT PF l). iDestruct 1 as (?) "[Hb _]". by iApply (ty_aligned with "Hb"). Qed.
+  Next Obligation. iIntros (it PT PF v). iDestruct 1 as (?) "[Hb _]". by iApply (ty_size_eq with "Hb"). Qed.
+  Next Obligation.
+    iIntros (it PT PF v). iDestruct 1 as (?) "[Hb ?]".
+    iDestruct (ty_deref with "Hb") as (?) "[? ?]". eauto with iFrame.
+  Qed.
+  Next Obligation.
+    iIntros (it PT PF l v ?) "Hl". iDestruct 1 as (?) "[Hb ?]".
+    iDestruct (ty_ref with "[] Hl Hb") as "?" => //. iExists _. iFrame.
+  Qed.
+
+End atomic_bool.
+
+Section programs.
+  Context `{!typeG Σ}.
+
+  Lemma subsume_atomic_bool_own_int l n it PT PF T:
+    (∃ b, subsume (l ◁ₗ n @ int it) (l ◁ₗ b @ boolean it) ((if b then PT else PF) ∗ T)) -∗
+    subsume (l ◁ₗ n @ int it) (l ◁ₗ atomic_bool it PT PF) T.
+  Proof.
+    iDestruct 1 as (b) "Hsub". iIntros "Hl".
+    iDestruct ("Hsub" with "Hl") as "[? [? $]]".
+    iExists _. by iFrame.
+  Qed.
+  Global Instance subsume_atomic_bool_own_int_inst l n it PT PF:
+    Subsume (l ◁ₗ n @ int it)%I (l ◁ₗ atomic_bool it PT PF) :=
+    λ T, i2p (subsume_atomic_bool_own_int l n it PT PF T).
+
+  Lemma i2v_bool_length b it:
+    length (i2v (Z_of_bool b) it) = it_length it.
+  Proof. by have /val_of_int_length -> := val_of_int_bool b it. Qed.
+  Lemma i2v_bool_Some b it:
+    val_to_int (i2v (Z_of_bool b) it) it = Some (Z_of_bool b).
+  Proof. apply val_to_of_int. apply val_of_int_bool. Qed.
+
+  Lemma type_write_atomic_bool l β it PT PF v ty `{!Movable ty} T:
+    (∃ b, subsume (v ◁ᵥ ty) (v ◁ᵥ b @ boolean it) (⌜ty.(ty_layout) = it⌝ ∗ (if b then PT else PF) ∗ T (atomic_bool it PT PF))) -∗
+    typed_write_end true v ty l β (atomic_bool it PT PF) T.
+  Proof.
+    iIntros "HT Hl Hv". iDestruct "HT" as (bnew) "Hsub".
+    iDestruct ("Hsub" with "Hv") as "(Hnew&->&Hif'&HT)".
+    destruct β.
+    - iDestruct "Hl" as (bold) "[Hl Hif]".
+      iMod (fupd_intro_mask' _ ∅) as "Hc" => //. iModIntro.
+      iDestruct (ty_aligned with "Hl") as %?.
+      iDestruct (ty_deref with "Hl") as (vb) "[Hmt Hold]".
+      iDestruct (ty_size_eq with "Hold") as %?.
+      iSplitL "Hmt". by iExists _; iFrame.
+      iIntros "!# Hl". iMod "Hc". iModIntro.
+      iExists _. iFrame. iExists bnew. iFrame.
+      iApply (@ty_ref with "[] Hl") => //. done.
+    - iDestruct "Hl" as (?) "#Hinv".
+      iInv "Hinv" as (b) "[>Hmt Hif]" "Hc".
+      iMod (fupd_intro_mask' _ ∅) as "Hc2". solve_ndisj. iModIntro.
+      iSplitL "Hmt".
+      { iExists _; iFrame; iPureIntro; split => //. apply i2v_bool_length. }
+      iIntros "!# Hl". iMod "Hc2".
+      iMod ("Hc" with "[Hif' Hl Hnew]").
+      { iModIntro. iExists bnew. iFrame. rewrite /i2v. by iDestruct "Hnew" as %->. }
+      iModIntro. iExists _. iFrame. by iSplit.
+  Qed.
+  Global Instance type_write_atomic_bool_inst l β it PT PF v ty `{!Movable ty}:
+    TypedWriteEnd true v ty l β (atomic_bool it PT PF) | 10 :=
+    λ T, i2p (type_write_atomic_bool l β it PT PF v ty T).
+
+  Lemma type_cas_atomic_bool (l : loc) β it PT PF lexp Pexp vnew Pnew T:
+    (∃ bexp bnew, subsume Pexp (lexp ◁ₗ bexp @ boolean it) (
+                  subsume Pnew (vnew ◁ᵥ bnew @ boolean it) ( ⌜it_length it ≤ loc_size⌝%nat ∗ (
+        ((if bexp then PT else PF) -∗ (if bnew then PT else PF) ∗ (
+            l ◁ₗ{β} atomic_bool it PT PF -∗ lexp ◁ₗ bexp @ boolean it -∗
+              T (val_of_bool true) (t2mt (true @ boolean bool_it)))) ∧
+            (l ◁ₗ{β} atomic_bool it PT PF -∗ lexp ◁ₗ negb bexp @ boolean it -∗
+                             T (val_of_bool false) (t2mt (false @ boolean bool_it)))
+    )))) -∗
+    typed_cas (IntOp it) l (l ◁ₗ{β} (atomic_bool it PT PF))%I lexp Pexp vnew Pnew T.
+  Proof.
+    iDestruct 1 as (bexp bnew) "Hsub". iIntros "Hl Hlexp Hvnew".
+    iDestruct ("Hsub" with "Hlexp") as "[Hlexp Hsub]".
+    iDestruct ("Hsub" with "Hvnew") as "[Hvnew [% Hsub]]".
+    iIntros (Φ) "HΦ".
+    (* TODO: don't unfold here *)
+    rewrite {1 2}/boolean/boolean_inner_type/int_inner_type/=.
+    iDestruct "Hlexp" as (ve Hve Hle) "He" => /=.
+    iDestruct "Hvnew" as %Hvnew.
+    destruct β.
+    - iDestruct "Hl" as (b) "[Hb Hif]".
+      (* TODO: don't unfold here *)
+      rewrite {1}/boolean/boolean_inner_type/int_inner_type/=.
+      iDestruct "Hb" as (vb Hvb Hlb) "Hb" => /=.
+      destruct (decide (b = bexp)); subst.
+      + iApply (wp_cas_suc with "Hb He") => //; try by [apply val_to_of_loc]; try by [apply val_to_of_int]; try by [apply: val_of_int_length].
+        iIntros "!# Hb Hexp".
+        iDestruct "Hsub" as "[Hsub _]". iDestruct ("Hsub" with "Hif") as "[Hif HT]".
+        iApply "HΦ". 2: iApply ("HT" with "[Hb Hif]"). done.
+        * iExists bnew. iFrame "Hif". iExists _. by iFrame.
+        * iExists _. by iFrame.
+      + iApply (wp_cas_fail with "Hb He") => //; try by [apply val_to_of_loc]; try by [apply val_to_of_int]; try by [apply: val_of_int_length]; try by [destruct b,bexp].
+        iIntros "!# Hb Hexp".
+        iDestruct "Hsub" as "[_ HT]".
+        iApply "HΦ". 2: iApply ("HT" with "[Hb Hif]"). done.
+        * iExists b. iFrame "Hif". iExists _. by iFrame.
+        * iExists _. iFrame. by destruct b, bexp.
+    - iDestruct "Hl" as (?) "#Hinv".
+      iApply (@wp_atomic).
+      iMod (inv_acc with "Hinv") as "[Hb Hc]" => //. iModIntro.
+      iDestruct "Hb" as (b) "[>Hmt Hif]".
+      destruct (decide (b = bexp)); subst.
+      + iApply (wp_cas_suc with "Hmt He") => //; try by [apply val_to_of_loc]; try by [apply val_to_of_int]; try by [apply: val_of_int_length]; try by [apply i2v_bool_Some].
+        iIntros "!# Hb Hexp".
+        iDestruct "Hsub" as "[Hsub _]". iDestruct ("Hsub" with "Hif") as "[Hif HT]".
+        iMod ("Hc" with "[Hb Hif]") as "_"; iModIntro. by iExists bnew; iFrame; rewrite /i2v Hvnew.
+        iApply "HΦ". 2: iApply ("HT" with "[]"). done.
+        * by iSplit.
+        * iExists _. by iFrame.
+      + iApply (wp_cas_fail with "Hmt He") => //; try by [apply val_to_of_loc]; try by [apply val_to_of_int]; try by [apply i2v_bool_Some]; try by [apply: val_of_int_length]; try by [destruct b,bexp].
+        iIntros "!# Hb Hexp".
+        iDestruct "Hsub" as "[_ HT]".
+        iMod ("Hc" with "[Hb Hif]") as "_"; iModIntro. by iExists b; iFrame; rewrite /i2v Hvnew.
+        iApply "HΦ". 2: iApply ("HT" with "[]"). done.
+        * by iSplit.
+        * iExists _. iFrame. rewrite val_of_int_bool. by destruct b, bexp.
+  Qed.
+  Global Instance type_cas_atomic_bool_inst (l : loc) β it PT PF (lexp : loc) Pexp vnew Pnew:
+    TypedCas (IntOp it) l (l ◁ₗ{β} (atomic_bool it PT PF))%I lexp Pexp vnew Pnew :=
+    λ T, i2p (type_cas_atomic_bool l β it PT PF lexp Pexp vnew Pnew T).
+
+End programs.
+
+Typeclasses Opaque atomic_bool.
